Aesop/Forward/State/ApplyGoalDiff.lean
@@ -1,0 +1,41 @@
+/-
+Copyright (c) 2024 Jannis Limperg. All rights reserved.
+Released under Apache 2.0 license as described in the file LICENSE.
+Authors: Jannis Limperg
+-/
+
+import Aesop.Forward.State
+import Aesop.RuleSet
+
+namespace Aesop
+
+open Lean Lean.Meta
+
+variable [Monad m] [MonadRulePatternCache m] [MonadControlT MetaM m]
+  [MonadLiftT MetaM m]
+
+-- FIXME rule pattern instantiation from the target are currently not
+-- considered.
+
+/-- Apply a goal diff to the state, adding and removing hypotheses as indicated
+by the diff. `goal` must be the post-goal of `diff`. -/
+def ForwardState.applyGoalDiff (rs : LocalRuleSet) (goal : MVarId)
+    (diff : GoalDiff) (fs : ForwardState) :
+    m (ForwardState × Array ForwardRuleMatch) :=
+  goal.withContext do
+    if ! diff.fvarSubst.isEmpty then
+      show MetaM _ from throwError "aesop: internal error: non-empty FVarSubst in GoalDiff is currently not supported"
+    let mut fs := fs
+    let mut ruleMatches := #[]
+    for h in diff.removedFVars do
+      fs := fs.eraseHyp h
+    for h in diff.addedFVars do
+      let rules ← rs.applicableForwardRules (← h.getType)
+      let patInsts ← rs.forwardRulePatternInstantiationsInLocalDecl (← h.getDecl)
+      let (fs', ruleMatches') ←
+        fs.addHypWithPatInstsCore ruleMatches goal h rules patInsts
+      fs := fs'
+      ruleMatches := ruleMatches'
+    return (fs, ruleMatches)
+
+end Aesop
